in_progress.v
@@ -1182,3 +1182,11 @@ Qed.
 End SecondSeparationTheorem.
 
 End SeparationTheorems.
+
+(* Next step: we need to show that for the rounding modes of interest,
+   the only discontinuities of those rounding modes are elements of
+   binary_float p for the directed rounding modes, and binary_float p+1
+   for the round-to-nearest rounding modes. *)
+
+
+   
